src/lang/Configuration.v
@@ -78,7 +78,6 @@ Module Threads.
       + apply TView.bot_wf.
       + apply TView.bot_closed.
       + ii. rewrite Memory.bot_get in LHS. congr.
-      + apply Memory.bot_finite.
   Qed.
 
   Lemma init_consistent syn: consistent (init syn) TimeMap.bot Memory.init.
