src/lang/Local.v
@@ -176,7 +176,6 @@ Module Local.
       (TVIEW_WF: TView.wf lc.(tview))
       (TVIEW_CLOSED: TView.closed lc.(tview) mem)
       (PROMISES: Memory.le lc.(promises) mem)
-      (FINITE: Memory.finite lc.(promises))
   .
   Hint Constructors wf.
 
