src/opt/ReorderRelFence.v
@@ -76,7 +76,6 @@ Proof.
   i. des.
   exploit Memory.promise_future; try apply PROMISE_SRC; eauto.
   { apply WF1_SRC. }
-  { apply WF1_SRC. }
   { SimPromises.none_if_tac; econs; ss. inv CLOSED.
     eapply sim_memory_closed_opt_view; eauto. }
   i. des.
@@ -176,7 +175,6 @@ Proof.
     try exact MEM1; try apply LOCAL1; eauto.
   { econs. ss. }
   { apply WF1_SRC. }
-  { apply WF1_TGT. }
   { apply WF1_TGT. }
   i. des. esplits.
   - econs; eauto.
